theories/Dijkstra/EuttEv.v
@@ -56,10 +56,17 @@ Inductive euttEvF
   | EqTauR : forall (ot1 : itree' E1 R1) (t2 : itree E2 R2),
       euttEvF vclo sim ot1 (observe t2) -> euttEvF vclo sim ot1 (TauF t2)
   | EqVis : forall (A B : Type) (e1 : E1 A) (e2 : E2 B ) (k1 : A -> itree E1 R1) (k2 : B -> itree E2 R2),
-      REv e1 e2 ->
+      REv e1 e2 -> 
       (forall (a : A) (b : B), RAns e1 a e2 b -> vclo sim (k1 a) (k2 b) : Prop) -> euttEvF vclo sim (VisF e1 k1) (VisF e2 k2).
 (*what if RE is empty? this definition seems to have serious problems*) 
 Hint Constructors euttEvF.
+(*
+Rev := fun _ _ => True
+Rans := fun _ _ _ _ => True
+RR := eq
+EqVis (Vis e1 Ret 0) (Vis e2 Ret 1)
+*)
+
 Definition euttEv_ (vclo : (itree E1 R1 -> itree E2 R2 -> Prop) -> itree E1 R1 -> itree E2 R2 -> Prop )
            (sim : itree E1 R1 -> itree E2 R2 -> Prop) (t1 : itree E1 R1) (t2 : itree E2 R2) :=
   euttEvF vclo sim (observe t1) (observe t2).
@@ -70,15 +77,65 @@ Proof.
   intros. red in H. red. intros. red. red in IN. induction IN; eauto.
 Qed.
 
-Hint Resolve euttEv_monot.
+
 
 Lemma euttEv_id_monot : monotone2 (@id (itree E1 R1 -> itree E2 R2 -> Prop) ).
 Proof. auto. Qed.
  
-Hint Resolve euttEv_id_monot.
+
 
 Definition euttEv : itree E1 R1 -> itree E2 R2 -> Prop := paco2 (euttEv_ id) bot2.
 
 End EuttEvF.
 
 
+Hint Resolve euttEv_monot : paco.
+
+Hint Resolve euttEv_id_monot : paco.
+
+Lemma euttEv_inv_tauL {E1 E2 R1 R2 REv RAns RR} t1 t2 :
+  @euttEv E1 E2 R1 R2 REv RAns RR (Tau t1) t2 -> euttEv REv RAns RR t1 t2.
+Proof.
+  intros. punfold H. red in H. simpl in *.
+  remember (TauF t1) as tt1. genobs t2 ot2.
+  hinduction H before t1; intros; try discriminate.
+  - inv Heqtt1. pclearbot. pstep. red. simpobs. econstructor; eauto. pstep_reverse.
+  - inv Heqtt1. punfold_reverse H.
+  - red in IHeuttEvF. pstep. red; simpobs. econstructor; eauto. pstep_reverse.
+Qed.
+
+Lemma euttEv_add_tauL {E1 E2 R1 R2 REv RAns RR} t1 t2 :
+  @euttEv E1 E2 R1 R2 REv RAns RR t1 t2 -> euttEv REv RAns RR (Tau t1) t2.
+Proof.
+  intros. pfold. red. cbn. constructor. pstep_reverse.
+Qed.
+
+Lemma euttEv_inv_tauR {E1 E2 R1 R2 REv RAns RR} t1 t2 :
+  @euttEv E1 E2 R1 R2 REv RAns RR t1 (Tau t2) -> euttEv REv RAns RR t1 t2.
+Proof.
+  intros. punfold H. red in H. simpl in *.
+  pstep. red. dependent induction H; subst; auto.
+  - pclearbot. rewrite <- x. constructor.
+    pstep_reverse.
+  - rewrite <- x. constructor. eapply IHeuttEvF; eauto.
+Qed.
+
+Lemma euttEv_add_tauR {E1 E2 R1 R2 REv RAns RR} t1 t2 :
+  @euttEv E1 E2 R1 R2 REv RAns RR t1 t2 -> euttEv REv RAns RR t1 (Tau t2).
+Proof.
+  intros. pfold. red. cbn. constructor. pstep_reverse.
+Qed.
+
+Lemma euttEv_inv_tauLR  {E1 E2 R1 R2 REv RAns RR} t1 t2 :
+   @euttEv E1 E2 R1 R2 REv RAns RR (Tau t1) (Tau t2) -> euttEv REv RAns RR t1 t2.
+Proof.
+  intros. punfold H. red in H. cbn in H. pstep. red.
+  dependent induction H.
+  - pclearbot. pstep_reverse.
+  - inv H; auto.
+    + pclearbot. constructor. pstep_reverse.
+    + constructor. eapply IHeuttEvF; eauto.
+  - inv H; auto.
+    + pclearbot. constructor. pstep_reverse.
+    + constructor. eapply IHeuttEvF; eauto.
+Qed.
